Hoare/SoundnessForBasicBlocks.thy
@@ -144,130 +144,6 @@ method set_solve =
    apply(rename_tac pair)
    apply(case_tac pair; clarsimp)*)
 
-
-lemma inst_arith_2_1_low_sound:
-notes
-  if_split[split del]
-shows
-"i = MUL \<or> i = DIV \<or> i = MOD \<Longrightarrow>
- triple_inst_sem
-  (\<langle> h \<le> 1022 \<and> Glow \<le> g \<and> 0 \<le> m \<rangle> \<and>*
-   continuing \<and>* memory_usage m \<and>* program_counter n \<and>*
-   stack_height (Suc (Suc h)) \<and>* stack (Suc h) v \<and>* stack h w \<and>* gas_pred g \<and>* rest)
-  (n, Arith i)
-  (program_counter (n + 1) \<and>* continuing \<and>* memory_usage m \<and>* stack_height (Suc h) \<and>*
-   stack h (arith_2_1_low i v w) \<and>* gas_pred (g - Glow) \<and>* rest)"
-apply(simp add: triple_inst_sem_def program_sem.simps as_set_simps)
-apply(clarify)
-apply(sep_simp simp: evm_sep; simp)
-apply(simp split: instruction_result.splits)
-apply(simp add: stateelm_means_simps stateelm_equiv_simps)
-apply(simp add: vctx_next_instruction_def)
-apply(case_tac i; clarsimp simp add: instruction_simps)
-  apply((sep_simp simp: evm_sep)+)
-  apply(simp add: stateelm_means_simps stateelm_equiv_simps)
-  apply(set_solve_arith_2_low)
- apply((sep_simp simp: evm_sep)+)
- apply(simp add: stateelm_means_simps stateelm_equiv_simps)
- apply(rule conjI)
-  apply(set_solve_arith_2_low)
-  apply(case_tac "w=0"; simp)
- apply(case_tac "w=0"; simp)
-apply((sep_simp simp: evm_sep)+)
-apply(simp add: stateelm_means_simps stateelm_equiv_simps)
-apply(rule conjI)
- apply(set_solve_arith_2_low)
-apply(case_tac "w=0"; simp)+
-done
-
-lemma inst_arith_2_1_verylow_sound:
-notes
-  if_split[split del]
-shows
-"i = ADD \<or> i = SUB \<or> i = inst_GT \<or> i = inst_EQ \<or> i = inst_LT \<Longrightarrow>
- triple_inst_sem
-  (\<langle> h \<le> 1022 \<and> Gverylow \<le> g \<and> 0 \<le> m \<rangle> \<and>*
-   continuing \<and>* memory_usage m \<and>* program_counter n \<and>* stack_height (Suc (Suc h)) \<and>*
-   stack (Suc h) v \<and>* stack h w \<and>* gas_pred g \<and>* rest)
-  (n, Arith i)
-  (program_counter (n + 1) \<and>* continuing \<and>* memory_usage m \<and>* stack_height (Suc h) \<and>*
-   stack h (arith_2_1_verylow i v w) \<and>* gas_pred (g - Gverylow) \<and>* rest)"
-apply(case_tac i; simp)
-    apply(inst_sound_set_eq)
-    apply(set_solve)
-   apply(inst_sound_set_eq)
-   apply(set_solve)
-  apply(inst_sound_set_eq)
-  apply(set_solve)
- apply(inst_sound_set_eq)
- apply(set_solve)
-apply(inst_sound_set_eq)
-apply(set_solve)
-done
-
-lemma inst_arith_3_1_sound:
-notes
-  if_split[split del]
-shows
-"i = ADDMOD \<or> i = MULMOD \<Longrightarrow>
- triple_inst_sem
-  (\<langle> h \<le> 1021 \<and> Gmid \<le> g \<and> 0 \<le> m \<rangle> \<and>*
-   continuing \<and>* memory_usage m \<and>* program_counter n \<and>*
-   stack_height (Suc (Suc (Suc h))) \<and>* stack (Suc (Suc h)) u \<and>*
-   stack (Suc h) v \<and>* stack h w \<and>* gas_pred g \<and>* rest)
-  (n, Arith i)
-  (program_counter (n + 1) \<and>* continuing \<and>* memory_usage m \<and>*
-   stack_height (Suc h) \<and>* stack h (arith_3_1 i u v w) \<and>*
-   gas_pred (g - Gmid) \<and>* rest)"
-apply(simp add: triple_inst_sem_def program_sem.simps as_set_simps)
-apply(clarify)
-apply(sep_simp simp: evm_sep; simp)
-apply(simp split: instruction_result.splits)
-apply(simp add: stateelm_means_simps stateelm_equiv_simps)
-apply(simp add: vctx_next_instruction_def)
-apply(case_tac i; clarsimp simp add: instruction_simps)
- apply((sep_simp simp: evm_sep)+)
- apply(simp add: stateelm_means_simps stateelm_equiv_simps)
- apply(rule conjI)
-  apply(erule_tac P="(_ \<and>* _)" in back_subst)
-  apply(set_solve)
-  apply(case_tac "w=0"; clarsimp)
- apply(case_tac "w=0"; clarsimp)
-apply((sep_simp simp: evm_sep)+)
-apply(simp add: stateelm_means_simps stateelm_equiv_simps)
-apply(rule conjI)
- apply(erule_tac P="(_ \<and>* _)" in back_subst)
- apply(set_solve)
- apply(case_tac "w=0"; clarsimp)
-apply(case_tac "w=0"; clarsimp)
-done
-
-lemma inst_bits_2_1_sound:
-"i = inst_AND \<or> i = inst_OR \<or> i = inst_XOR \<or> i = BYTE \<Longrightarrow>
- triple_inst_sem
-  (\<langle> h \<le> 1022 \<and> Gverylow \<le> g \<and> 0 \<le> m \<rangle> \<and>*
-   continuing \<and>*
-   memory_usage m \<and>*
-   program_counter n \<and>*
-   stack_height (Suc (Suc h)) \<and>*
-   stack (Suc h) v \<and>* stack h w \<and>* gas_pred g \<and>* rest)
-  (n, Bits i)
-  (program_counter (n + 1) \<and>*
-   continuing \<and>*
-   memory_usage m \<and>*
-   stack_height (Suc h) \<and>*
-   stack h (bits_2_1_verylow i v w) \<and>* gas_pred (g - Gverylow) \<and>* rest)"
-apply(case_tac i; simp)
-   apply(inst_sound_set_eq)
-   apply(set_solve)
-  apply(inst_sound_set_eq)
-  apply(set_solve)
- apply(inst_sound_set_eq)
- apply(set_solve)
-apply(inst_sound_set_eq)
-apply(set_solve)
-done
-
 (* From HoareTripleForInstructions2 *)
 lemma tmp001:
 "length lst = h \<Longrightarrow>
@@ -320,13 +196,20 @@ notes
   if_split[split del]
 shows
 "triple_inst_sem
-  (\<langle> h \<le> 1024 \<and> Suc (unat n) < h \<and> Gverylow \<le> g \<and> 0 \<le> m \<rangle> \<and>*
-   stack_height h \<and>* stack (h - Suc 0) w \<and>* stack (h - Suc (Suc (unat n))) v \<and>*
-   program_counter k \<and>* gas_pred g \<and>* memory_usage m \<and>* continuing \<and>* rest)
-  (k, Swap n)
-  (program_counter (k + 1) \<and>* gas_pred (g - Gverylow) \<and>*
-   stack_height h \<and>* stack (h - Suc 0) v \<and>* stack (h - Suc (Suc (unat n))) w \<and>*
-   memory_usage m \<and>* continuing \<and>* rest)"
+        (\<langle> h \<le> 1023 \<and>
+           Suc (unat n) \<le> h \<and> Gverylow \<le> g \<and> 0 \<le> m \<rangle> \<and>*
+         stack_height (Suc h) \<and>*
+         stack h w \<and>*
+         stack (h - unat n - 1) v \<and>*
+         program_counter k \<and>*
+         gas_pred g \<and>* memory_usage m \<and>* continuing \<and>* rest)
+        (k, Swap n)
+        (program_counter (k + 1) \<and>*
+         gas_pred (g - Gverylow) \<and>*
+         stack_height (Suc h) \<and>*
+         stack h v \<and>*
+         stack (h - unat n - 1) w \<and>*
+         memory_usage m \<and>* continuing \<and>* rest)"
 apply(simp add: triple_inst_sem_def program_sem.simps as_set_simps)
 apply(clarify)
 apply(sep_simp simp: evm_sep; simp)
@@ -339,41 +222,602 @@ apply(simp add: stateelm_means_simps stateelm_equiv_simps)
 apply(rule conjI)
  apply(erule_tac P="(_ \<and>* _)" in back_subst)
  apply(rule equalityI; rule subsetI)
- apply(clarsimp)
+ 		apply(clarsimp)
  apply(rename_tac elm; simp add: as_set_simps)
- apply(case_tac elm; simp add: instruction_result_as_set_def stateelm_equiv_simps)
- apply(rename_tac pair)
- apply(case_tac pair; simp add: stateelm_equiv_simps)
- apply(simp add: rev_append_eq)
- apply(rule conjI)
-  apply(split if_split; rule conjI; clarsimp simp add: rev_drop)
-  apply(simp add: rev_append_eq split: if_split)
-  apply(rule conjI)
-   apply(simp add: take_drop_nth)
-  apply(clarsimp simp add: rev_nth)
-  apply(rule arg_cong[where f="\<lambda>x. _ ! x"], arith)
- apply(auto)[1]
-apply(clarsimp)
- apply(rename_tac elm; simp add: as_set_simps)
- apply(case_tac elm; simp add: instruction_result_as_set_def stateelm_equiv_simps)
- apply(rename_tac pair)
- apply(case_tac pair; simp add: stateelm_equiv_simps)
- apply(simp add: rev_append_eq)
-  apply(split if_split; rule conjI; clarsimp simp add: rev_drop)
-   apply(arith)
-  apply(simp add: rev_nth rev_append_eq nth_append)
-  apply(split if_split; rule conjI; clarsimp simp add: rev_drop)
-  apply(subgoal_tac "aa < length (vctx_stack x1) - Suc 0")
-   apply(simp add: take_drop_nth, simp add: rev_nth)
-  apply(thin_tac "aa < _", arith)
- apply(drule leI)+
- apply(erule impE)
-  apply(arith)
- apply(simp)
-apply(simp add: rev_nth)
+ apply(case_tac elm; clarsimp simp add: instruction_result_as_set_def stateelm_equiv_simps)
+ 		apply(rename_tac pair)
+ 		apply(case_tac "pair = length t - Suc (unat n)")
+ 		 apply(simp)
+ 		apply(clarsimp)
+ 		apply(case_tac "Suc (unat n) = length t")
+ 		 apply(clarsimp simp add: min_def short_rev_append)
+ 		 apply(simp add: rev_take rev_append_eq)
+ 		apply(simp add: rev_take rev_append_eq min_def)
+ 		apply(subgoal_tac "length t > 0"; clarsimp)
+ 		apply(split if_splits; clarsimp)
+ 		 apply(simp add: rev_nth)
+ 		 apply(subst (asm) Suc_diff_Suc)
+ 			apply(arith)
+ 		 apply(simp)
+ 		apply(simp add: rev_nth not_less nth_append split: if_splits)
+ 	 apply(clarsimp simp add: as_set_simps)
+ 	 apply(rename_tac elm, case_tac elm; simp)
+ 	  apply(clarsimp)
+ 	apply(rename_tac pair)
+ 		 		apply(case_tac "pair = length t - Suc (unat n)")
+ 		 apply(simp)
+ 		apply(clarsimp)
+ (* apply(case_tac pair; simp add: stateelm_equiv_simps) *)
+ 		apply(case_tac "Suc (unat n) = length t")
+ 		 apply(clarsimp simp add: min_def short_rev_append)
+ 		 apply(simp add: rev_take rev_append_eq)
+ 		apply(simp add: rev_take rev_append_eq min_def)
+ 		apply(subgoal_tac "length t > 0"; clarsimp)
+ 		apply(split if_splits; clarsimp)
+ 		 apply(simp add: rev_nth)
+ 		 apply(subst (asm) Suc_diff_Suc)
+ 			apply(arith)
+ 		 apply(simp)
+ 		apply(simp add: rev_nth not_less nth_append split: if_splits)
 apply(arith)
 done
+		
+		lemma variable_context_pc_change:
+"variable_ctx_as_set (x1\<lparr>vctx_pc := vctx_pc x1 + 1\<rparr>) = insert (PcElm (vctx_pc x1 + 1)) (variable_ctx_as_set x1) - {PcElm (vctx_pc x1)}"
+by (auto simp add: as_set_simps)
 
+	lemma memory_elm_in_memory_range_elms:
+	"x \<in> memory_range_elms memaddr v \<Longrightarrow> \<exists>a b. x = MemoryElm (a, b)"
+	apply(induction v arbitrary: memaddr; simp)
+	apply(erule disjE; simp)
+	done
+
+lemma memory_elm_in_memory_range_elms':
+	"\<forall>a b. x \<noteq> MemoryElm (a,b) \<Longrightarrow> x \<notin> memory_range_elms m v"
+	apply(rule notI)
+	apply(drule memory_elm_in_memory_range_elms)
+	apply(simp)
+	done
+		
+		lemma memory_range_pc_update :
+  "x \<in> memory_range_elms in_begin input \<Longrightarrow>
+   x \<in> variable_ctx_as_set
+               (x1
+                \<lparr>vctx_pc := p \<rparr>) =
+   (x \<in> variable_ctx_as_set x1)"
+   by (auto simp: as_set_simps dest: memory_range_elms_all)
+	
+lemmas memory_range_elms_set_simps=
+	memory_range_elms_in_c
+	memory_range_in_minus_balance_as
+	memory_range_in_union_balance
+	memory_range_constant_union
+	memory_range_in_caller
+	memory_range_in_coinbase
+	memory_range_insert_cont
+	memory_range_elms_in_insert_continuing
+	memory_range_elms_in_insert_contract_action
+	memory_range_elms_in_insert_gas
+	memory_range_elms_in_mu
+	memory_range_in_origin
+	memory_range_in_pc
+	memory_range_in_sent_value
+	not_memory_range_elms_all
+	memory_range_elms_i
+	memory_range_advance
+	memory_range_elms_in_minus_statck_topmost
+	memory_range_elms_logs_update
+	memory_range_elms_update_balance
+	memory_range_elms_update_memory_usage
+	memory_gane_elms_in_stack_update
+	memory_range_in_minus_balance
+	memory_range_elms_in_x_minus_lognum
+	memory_range_elms_in_minus_continuing
+	memory_range_elms_in_minus_gas
+	memory_range_elms_in_minus_mu
+	memory_range_elms_in_minus_stack
+	memory_range_elms_in_minus_stackheight
+	memory_range_elms_in_minus_this
+	memory_range_elms_not_account_existence
+	memory_range_elms_not_code
+	memory_range_elms_not_pc
+	memory_range_elms_not_continuing
+	memory_range_continue
+	memory_range_advance_pc
+	memory_range_balance
+	memory_range_gas_update
+	memory_range_memory_usage
+	memory_range_stack
+	memory_range_elms_cut_memory
+	memory_elm_in_memory_range_elms
+	memory_elm_in_memory_range_elms'
+	memory_range_elms_all
+	memory_range_pc_update
+	
+lemma inst_mload_sound :
+notes
+  unat_bintrunc[simp del]
+shows
+"triple_inst_sem
+  (\<langle> h \<le> 1023  \<and> g \<ge> Gverylow - Cmem memu + Cmem (M memu memaddr 32) \<and> memu \<ge> 0 \<and>
+    length (word_rsplit v::byte list) = unat (32::w256)\<rangle> \<and>*
+   stack h memaddr \<and>* stack_height (Suc h) \<and>* program_counter n \<and>*   
+   memory_usage memu \<and>* memory memaddr v \<and>* gas_pred g \<and>* continuing \<and>* rest)
+  (n, Memory MLOAD)
+  (program_counter (n + 1) \<and>* stack_height (Suc h) \<and>* stack h v \<and>*
+   memory memaddr v \<and>* memory_usage (M memu memaddr 32) \<and>*
+   gas_pred (g - Gverylow + Cmem memu - Cmem (M memu memaddr 32)) \<and>*
+   continuing \<and>* rest)"
+apply(simp add: triple_inst_sem_def program_sem.simps as_set_simps instruction_sem_def)
+	apply(clarify)
+apply(simp add: memory_def)
+apply(sep_simp simp: pure_sep)
+apply(sep_simp simp: evm_sep; simp)
+apply(simp add: memory_range_sep)
+	apply(simp split: instruction_result.splits)
+	apply(simp add: stateelm_means_simps stateelm_equiv_simps)
+ 	apply(simp add: memory_range_elms_set_simps)
+	apply(cut_tac memory_range_elms_cut_memory[where lst="word_rsplit v"])
+	apply(drule spec2[where x=memaddr and y=32]; simp)
+		apply(drule mp, assumption)
+apply(simp add: vctx_next_instruction_def)
+apply(clarsimp)
+apply(simp add: instruction_simps vctx_stack_default_def del: Cmem_def M_def)
+	apply((sep_simp simp: evm_sep)+)
+apply(simp add: variable_context_pc_change)
+apply(simp add: read_word_from_bytes_def unat_bintrunc byte_list_fill_right_def word_rcat_rsplit)
+	apply(simp add: stateelm_means_simps stateelm_equiv_simps)
+apply(simp add: memory_range_elms_set_simps)
+	apply(rule conjI)
+apply(erule_tac P="(_ \<and>* _)" in back_subst)
+	 apply(set_solve)
+	apply(clarsimp)
+	 apply(simp add: memory_range_elms_set_simps)
+	  apply(fastforce)
+done
+
+	(*MSTORE*)
+lemma store_list_mem_gt:
+"unat (p - pos) \<ge> length lst \<Longrightarrow>
+ store_byte_list_memory pos lst orig p = orig p"
+apply(induction lst arbitrary: pos)
+ apply(simp add: store_byte_list_memory_def)
+apply(subst store_byte_list_memory_def)
+apply(simp split: option.splits)
+done
+
+lemma store_list_mem_ls:
+"unat (p - pos) < length lst \<Longrightarrow>
+ store_byte_list_memory pos lst orig p = lst ! unat (p-pos)"
+apply(induction lst arbitrary: pos)
+ apply(simp add: store_byte_list_memory_def)
+apply(subst store_byte_list_memory_def)
+apply(simp split: option.splits)
+done
+
+lemma tmp003:
+"n < 35 \<Longrightarrow> unat (x - p::w256) < n \<Longrightarrow> unat (x - p + 2) < Suc (Suc n)"
+apply(subgoal_tac "unat (x-p+2)-2 < n")
+ apply(auto)[1]
+ using unat_add_lem
+apply(insert unat_add_lem[where x="x-p" and y=2])[1]
+apply(drule iffD1)
+ apply(auto)
+done
+
+lemma  unat_minus_Suc:
+" 0 < unat (x - pos::w256) \<Longrightarrow> unat (x - pos) = Suc (unat (x - (pos + 1)))"
+apply(subgoal_tac "unat (1+ (x - (pos + 1))) = Suc (unat (x - (pos + 1)))")
+ apply(auto)[1]
+apply(rule unatSuc)
+apply(simp add: unat_gt_0)
+done
+
+lemma store_blst_mem_append:
+notes
+  if_split[split del]
+shows
+"length lst < 32 \<Longrightarrow>
+store_byte_list_memory pos (a # lst) orig =
+((store_byte_list_memory (pos+1) lst orig)(pos:=a))"
+apply(rule ext)
+apply(induction lst arbitrary: pos a)
+ apply(case_tac "unat (x - pos) < length [a]")
+  apply(clarsimp simp add: store_list_mem_ls unat_eq_0)
+ apply(clarsimp split: if_split)
+ apply(rule conjI)
+  apply(simp add: unat_gt_0)
+ apply(simp add: store_list_mem_gt)
+apply(case_tac "x=pos")
+ apply(simp add: store_list_mem_ls)
+apply(drule_tac x=x in meta_spec)
+apply(drule_tac x="pos + 1" and y="a" in meta_spec2)
+apply(drule meta_mp)
+ apply(simp)
+apply(clarsimp)
+apply(case_tac "x=pos+1")
+ apply(simp add: store_list_mem_ls)
+apply(clarsimp)
+apply(case_tac "unat (x-pos) < length (aa#a#lst)")
+ apply(simp add: store_list_mem_ls)
+ apply(drule sym)
+ apply(simp)
+ apply(subst store_list_mem_ls)
+  apply(simp)
+  apply(cut_tac pos=pos and x=x in unat_minus_Suc)
+   apply(simp add: unat_gt_0)
+  apply(simp)
+ apply(insert unatSuc)[1]
+ apply(drule_tac x="x - (pos + 1)" in meta_spec)
+ apply(simp)
+apply(simp add: store_list_mem_gt)
+apply(drule sym, simp)
+apply(subst store_list_mem_gt; simp)
+apply(simp add: not_less_eq)
+apply(cut_tac pos=pos and x=x in unat_minus_Suc)
+ apply(simp add: unat_gt_0)
+apply(simp)
+done
+
+lemma memory_as_set_append:
+"memory_as_set
+ (z(memaddr:=a)) =
+insert (MemoryElm (memaddr, a))
+(memory_as_set z - {MemoryElm (memaddr, z memaddr)})"
+apply(simp add: memory_as_set_def)
+apply(rule subset_antisym)
+ apply(rule subsetI)
+ apply(case_tac "x = (MemoryElm (memaddr, a))")
+  apply(clarsimp)
+ apply(clarsimp)
+apply(rule subsetI)
+apply(clarsimp)
+apply(erule disjE)
+ apply(simp)
+apply(erule conjE)
+apply(erule exE)
+apply(rule_tac x=aa in exI)
+apply(clarsimp)
+done
+
+lemma memory_elm_in_vctx:
+"(MemoryElm (a,b)
+   \<in> variable_ctx_as_set v) =
+(MemoryElm (a,b)
+   \<in> memory_as_set (vctx_memory v))"
+by (auto simp add: as_set_simps)
+
+lemma memory_range_elms_in_vctx:
+"(memory_range_elms memaddr lst
+   \<subseteq> variable_ctx_as_set v) =
+(memory_range_elms memaddr lst
+  \<subseteq> memory_as_set (vctx_memory v))"
+by (auto simp add: as_set_simps memory_range_elms_set_simps)
+
+lemma word_of_int_n0:
+"0 < k \<Longrightarrow> k < 2^256\<Longrightarrow> (word_of_int k::w256) \<noteq> 0"
+apply(subst zero_word_def)
+apply(subst word_of_int_inj; simp)
+done
+
+lemma ind_memory_rg_elms:
+"k > 0 \<Longrightarrow> k < 2^256 - int (length lst) \<Longrightarrow>
+MemoryElm (m, b) \<notin> memory_range_elms (m + word_of_int k) lst"
+apply(induction lst arbitrary:  k)
+ apply(simp)
+apply(rule notI)
+apply(simp)
+apply(simp add:word_of_int_n0)
+apply(drule_tac x="k+1" in meta_spec)
+apply(simp add: wi_hom_syms(5))
+apply(simp add: word_succ_p1)
+apply(subgoal_tac "m + word_of_int k + 1=m + (word_of_int k + 1)"; simp)
+done
+
+lemma memory_range_elms_in_store:
+"length lst \<le> unat (32::w256) \<Longrightarrow>
+memory_range_elms memaddr lst
+   \<subseteq> memory_as_set
+       (store_byte_list_memory memaddr lst mem)"
+apply(induction lst arbitrary: memaddr; simp)
+apply(rule context_conjI)
+ apply(simp add: store_byte_list_memory_def memory_as_set_def)
+apply(clarsimp)
+apply(case_tac x; clarsimp simp add: stateelm_means_simps stateelm_equiv_simps memory_range_elms_set_simps)
+apply(subst store_blst_mem_append, simp)
+apply(simp add:  memory_as_set_append)
+apply(case_tac "aa=memaddr")
+ apply(simp)
+ apply(cut_tac m=memaddr and k=1 and lst=lst and b=b in ind_memory_rg_elms; simp)
+apply(simp)
+apply(drule_tac x="memaddr + 1" in meta_spec)
+apply(drule rev_subsetD; simp)
+done
+
+lemma diff_set_commute_sing:
+"A - {b} - {c} = A - {c} - {b}"
+by(auto)
+
+lemma diff_memory_elms_commute_fst:
+"A - {b} - memory_range_elms x y = A - memory_range_elms x y - {b}"
+apply(induction y arbitrary: x; simp)
+apply(rule subset_antisym; rule subsetI)
+ apply(simp add: diff_set_commute_sing[where b="MemoryElm _"])+
+done
+
+lemma diff_memory_elms_commute_end:
+"A - memory_range_elms x y - {b} = A - {b} - memory_range_elms x y"
+apply(induction y arbitrary: x; simp)
+apply(rule subset_antisym; rule subsetI)
+ apply(simp add: diff_set_commute_sing[where b="MemoryElm _"])+
+done
+
+lemma memory_elms_out_of_range:
+"length v \<le> unat (a - m) \<Longrightarrow>
+ MemoryElm (a, b) \<notin> memory_range_elms m v"
+apply(induction v arbitrary: m; simp)
+apply(case_tac "a=m"; simp)
+apply(drule_tac x="m+1" in meta_spec)
+apply(drule meta_mp)
+ apply(cut_tac pos=m in unat_minus_Suc[where x=a]; simp)
+apply(simp)
+done
+
+lemma memory_elms_in_range:
+"length lst < 2^256 \<Longrightarrow>
+(unat (a - m) < length lst \<and>
+ lst ! unat (a - m) = x ) =
+ (MemoryElm (a, x) \<in> memory_range_elms m lst)"
+apply(rule iffI)
+apply(induction lst arbitrary: m; simp)
+apply(case_tac "a=m"; simp)
+apply(drule_tac x="m+1" in meta_spec)
+apply(drule meta_mp)
+  apply(cut_tac pos=m in unat_minus_Suc[where x=a];simp add: unat_gt_0)
+ apply(cut_tac pos=m in unat_minus_Suc[where x=a];simp add: unat_gt_0)
+apply(induction lst arbitrary: m; simp)
+apply(case_tac "a=m"; simp)
+ apply(erule disjE, simp)
+ apply(cut_tac m=m and k=1 and lst=lst and b=x in ind_memory_rg_elms; simp)
+apply(drule_tac x="m+1" in meta_spec)
+apply(drule meta_mp)
+  apply(cut_tac pos=m in unat_minus_Suc[where x=a];simp add: unat_gt_0)
+ apply(cut_tac pos=m in unat_minus_Suc[where x=a];simp add: unat_gt_0)
+  done
+  	
+  	lemma memory_elms_not_in_range:
+"length lst < 2^256 \<Longrightarrow>
+(MemoryElm (a, x) \<notin> memory_range_elms m lst) =
+(\<not>(unat (a - m) < length lst \<and>
+ lst ! unat (a - m) = x ))"
+ 			by(simp add: memory_elms_in_range)
+ 				
+lemma elm_in_range_in_lst:
+	"unat n < length lst \<Longrightarrow>
+ MemoryElm (m+ n, lst ! unat n) \<in> memory_range_elms m lst"
+	apply(induction lst arbitrary:n m; simp)
+	apply(subst disj_commute)
+	apply(rule disjCI)
+	apply(clarsimp)
+	apply(case_tac "n=0"; simp)
+		apply(drule_tac x="n - 1" and y="m+1" in meta_spec2)
+	apply(drule meta_mp)
+	 apply(simp add: unat_minus_one )
+	 apply(subst less_diff_conv2)
+	  apply(subst (asm) word_neq_0_conv)
+	  apply(subst (asm) word_less_nat_alt)
+	  apply(arith)
+	 apply(arith)
+	apply(simp add: unat_minus_one)
+		apply(subgoal_tac "unat n > 0"; simp)
+			  apply(simp add:  word_neq_0_conv word_less_nat_alt)
+	done
+		
+lemma in_mem_not_in_range:
+	"length lst < 2^256 \<Longrightarrow>
+	memory_range_elms m lst \<subseteq> memory_as_set (vctx_memory x) \<Longrightarrow>
+	MemoryElm (a, b) \<in> memory_as_set (vctx_memory x) \<Longrightarrow>
+	MemoryElm (a, b) \<notin> memory_range_elms m lst \<Longrightarrow>
+	unat (a - m) \<ge> length lst"
+	apply(simp add: memory_as_set_def)
+	apply(simp add: memory_elms_not_in_range)
+	apply(case_tac "length lst \<le> unat (a - m)"; simp)
+	apply(simp add: not_le)
+	apply(simp add: subset_eq Ball_def)
+	apply(insert elm_in_range_in_lst[where n="a-m" and m=m and lst=lst], simp)
+	apply(drule spec[where x="MemoryElm (a, lst ! unat (a - m))"])
+	apply(simp)
+	done
+		
+lemma vctx_memory_store_memory_set_eq:
+"length (word_rsplit v::byte list) < 2^256 \<Longrightarrow>
+memory_range_elms memaddr (word_rsplit old_v)
+    \<subseteq> memory_as_set (vctx_memory x1) \<Longrightarrow>
+    length (word_rsplit old_v::byte list) =  length (word_rsplit v::byte list) \<Longrightarrow>
+    memory_range_elms memaddr (word_rsplit v)
+    \<subseteq> memory_as_set (store_word_memory memaddr v (vctx_memory x1)) \<Longrightarrow>
+    contexts_as_set
+     (x1\<lparr>vctx_memory := store_word_memory memaddr v (vctx_memory x1)\<rparr>)
+     co_ctx -
+    memory_range_elms memaddr (word_rsplit v) =
+    contexts_as_set x1 co_ctx -
+    memory_range_elms memaddr (word_rsplit old_v)"
+apply(simp add: contexts_as_set_def)
+apply(rule subset_antisym; rule subsetI)
+	 apply(case_tac "\<exists>a b. x = MemoryElm (a,b)")
+	  apply(clarsimp simp add: memory_elm_not_constant memory_range_elms_set_simps)
+	  apply(simp add: memory_elms_not_in_range)
+	  apply(rule conjI)
+	  		apply(thin_tac " _ \<subseteq> _", thin_tac "_=_", thin_tac "_\<subseteq>_")
+		 apply(simp add: stateelm_means_simps stateelm_equiv_simps)
+		 apply(simp add: store_word_memory_def store_byte_list_memory_def)
+	apply(split option.splits; clarsimp)
+		apply(clarsimp)
+		apply(simp add: stateelm_means_simps stateelm_equiv_simps)
+ apply(simp add: store_word_memory_def store_byte_list_memory_def)
+ apply(rename_tac elm, case_tac elm; simp add: stateelm_means_simps memory_range_elms_set_simps stateelm_equiv_simps)
+ apply(simp add: as_set_simps)
+ 	 apply(simp add: as_set_simps)
+ 	  
+ 	apply(case_tac "\<exists>a b. x = MemoryElm (a,b)")
+ 	 prefer 2
+ 	  apply(rename_tac elm, case_tac elm; simp add: stateelm_means_simps memory_range_elms_set_simps stateelm_equiv_simps)
+ apply(simp add: as_set_simps)
+ apply(simp add: as_set_simps)
+
+	  apply(clarsimp simp add: memory_elm_not_constant memory_range_elms_set_simps)
+	apply(simp add: memory_elm_in_vctx)
+	apply(insert in_mem_not_in_range[where m=memaddr])
+		apply(drule_tac x="word_rsplit old_v::byte list" and y="x1"in meta_spec2)
+	apply(drule_tac x=a and y=b in meta_spec2)
+		apply(clarsimp)
+	apply(subst memory_elms_not_in_range, simp)
+	  		apply(thin_tac " _ \<subseteq> _", thin_tac "_=_", thin_tac "_\<subseteq>_")
+		 apply(simp add: memory_as_set_def)
+		 apply(simp add: store_word_memory_def store_byte_list_memory_def)
+done
+
+lemma memory_in_mem_as_set:
+"x \<in> memory_as_set m \<Longrightarrow> \<exists>a b. x= MemoryElm (a,b)"
+by(auto simp add: as_set_simps)
+
+
+lemma inst_mstore_sound :
+notes
+  unat_bintrunc[simp del]
+shows
+"triple_inst_sem
+  (\<langle> h \<le> 1022 \<and> g \<ge> Gverylow - Cmem memu + Cmem (M memu memaddr 32) \<and> memu \<ge> 0 \<and>
+    length (word_rsplit old_v::byte list) = unat (32::w256) \<and>
+    length (word_rsplit v::byte list) = unat (32::w256)\<rangle> \<and>*
+   stack (h+1) memaddr \<and>* stack h v \<and>* stack_height (h+2) \<and>*
+   program_counter n \<and>* memory_usage memu \<and>*
+   memory memaddr old_v \<and>* gas_pred g \<and>* continuing \<and>* rest)
+  (n, Memory MSTORE)
+  (program_counter (n + 1) \<and>* stack_height h \<and>* memory memaddr v \<and>* 
+   gas_pred (g - Gverylow + Cmem memu - Cmem (M memu memaddr 32)) \<and>*
+   memory_usage (M memu memaddr 32) \<and>* continuing \<and>* rest)"
+apply(simp add: triple_inst_sem_def program_sem.simps as_set_simps instruction_sem_def)
+apply(clarify)
+apply(simp add: memory_def)
+apply(sep_simp simp: pure_sep)
+	apply(sep_simp simp: evm_sep; simp, (erule conjE)?)+
+	apply(simp split: instruction_result.splits add: memory_range_sep)
+	apply(simp add: stateelm_means_simps stateelm_equiv_simps)
+apply(simp add: vctx_next_instruction_def)
+apply(clarsimp simp add: rev_nth)
+apply(simp add: instruction_simps vctx_stack_default_def del: Cmem_def M_def)
+apply(subst conj_commute, rule context_conjI)
+	apply(simp add: memory_range_elms_set_simps)
+	apply(simp add: store_word_memory_def memory_range_elms_in_vctx)
+  apply(simp only: memory_range_elms_in_store)
+apply(erule_tac P="(_ \<and>* _)" in back_subst)
+apply(simp add: diff_set_commute_sing[where c="ContinuingElm True"])
+	apply(simp add: diff_memory_elms_commute_fst  memory_range_elms_in_vctx)
+	apply(simp add: memory_range_elms_set_simps)
+	apply(rule subst[OF vctx_memory_store_memory_set_eq[where old_v=old_v and v=v]]; simp?)
+		apply(simp add:  memory_range_elms_in_vctx)
+		apply(simp add: store_word_memory_def memory_range_elms_in_store)
+		 apply(subgoal_tac "unat (32::w256) = 32"; simp add: unat_def)
+		apply(simp add: memory_range_elms_in_vctx)
+		apply(simp add: memory_range_elms_in_vctx)
+		 apply(simp add: diff_memory_elms_commute_end)
+apply(rule arg_cong[where f="\<lambda>u. u - memory_range_elms _ _"])
+apply(rule subset_antisym; rule subsetI)
+apply(simp add: memory_range_elms_set_simps)
+	 apply(case_tac "\<exists>a b. x= MemoryElm (a,b)"; clarsimp)
+	  	apply(simp add: stateelm_means_simps stateelm_equiv_simps)
+	 apply(case_tac x; clarsimp simp add: stateelm_means_simps stateelm_equiv_simps)
+	 apply(case_tac "a=length ta"; clarsimp)
+	 apply(case_tac "a<length ta"; clarsimp)
+	 apply(erule notE, simp add: short_rev_append)
+	apply(clarsimp)
+	apply(case_tac x; clarsimp simp add: stateelm_means_simps stateelm_equiv_simps)
+	apply(simp add: short_rev_append)
+	done
+		
+lemma inst_return_sem :
+notes
+  if_split[split del]
+shows
+  "triple_inst_sem
+    (\<langle> h \<le> 1022 \<and> m \<ge> 0 \<and> length lst = unat v \<and> (Cmem (M m u v) - Cmem m) \<le> g \<rangle> \<and>*
+     continuing \<and>* memory_usage m \<and>* memory_range u lst \<and>*
+     program_counter n \<and>* stack_height (Suc (Suc h)) \<and>* gas_pred g \<and>*
+     stack (Suc h) u \<and>* stack h v \<and>* rest)
+    (n, Misc RETURN)
+    (stack_height (Suc (Suc h)) \<and>* not_continuing \<and>* memory_usage (M m u v) \<and>*
+     action (ContractReturn lst) \<and>* gas_pred (g - (Cmem (M m u v) - Cmem m)) \<and>*
+     stack (Suc h) u \<and>* stack h v \<and>* memory_range u lst \<and>*
+     program_counter n \<and>* rest)"
+ apply(simp add: triple_inst_sem_def)
+ apply(simp add: program_sem.simps  as_set_simps instruction_sem_def)
+ apply(clarify)
+ apply(case_tac presult; clarsimp)
+   defer
+   apply(simp add: as_set_simps)
+   apply(sep_simp simp: continuing_sep; clarsimp)
+ apply(sep_simp simp: pure_sep)
+ 			apply(sep_simp simp: evm_sep, simp?, (erule conjE)?)+
+ 				 apply(simp add: instruction_simps vctx_returned_bytes_def)
+ 			apply(simp add: stateelm_means_simps stateelm_equiv_simps)
+ 				apply(simp add: memory_range_sep memory_range_elms_set_simps)
+ apply(clarify)
+ apply(clarsimp)
+ 			apply(simp add: instruction_simps)
+ 				apply(simp add: stateelm_means_simps stateelm_equiv_simps)
+ 				apply(simp add: vctx_returned_bytes_def memory_range_elms_cut_memory)
+ apply(rule conjI)
+ 			 apply(erule_tac P="(_ \<and>* _)" in back_subst)
+ 			  
+ 			 apply(auto simp add: as_set_simps )[1]
+ 			apply(thin_tac "(_ \<and>* _) _")
+  		apply(subst (asm) subset_eq)
+  		apply(simp add: Ball_def)
+  		apply(clarsimp simp add: memory_range_elms_set_simps)
+  			apply(drule_tac x=x in spec, simp)
+  		apply(drule memory_elm_in_memory_range_elms)
+  			apply(clarsimp)
+  		apply(simp add: stateelm_means_simps stateelm_equiv_simps)
+  done
+  	
+  	lemma inst_dup_sound:
+"triple_inst_sem
+        (\<langle> h \<le> 1023 \<and> unat n < h \<and> Gverylow \<le> g \<and> 0 < m\<rangle> \<and>*
+         stack_height h \<and>*
+         stack (h - unat n - 1) w \<and>*
+         memory_usage m \<and>*
+         program_counter k \<and>*
+         gas_pred g \<and>* continuing \<and>* rest)
+        (k, Dup n)
+        (program_counter (k + 1) \<and>*
+         gas_pred (g - Gverylow) \<and>*
+         stack_height (Suc h) \<and>*
+         stack (h - unat n - 1) w \<and>*
+         stack h w \<and>*
+         memory_usage m \<and>* continuing \<and>* rest)"
+apply(simp add: triple_inst_sem_def program_sem.simps as_set_simps)
+apply(clarify)
+apply(sep_simp simp: evm_sep; simp)
+apply(simp split: instruction_result.splits)
+apply(simp add: stateelm_means_simps stateelm_equiv_simps)
+apply(simp add: vctx_next_instruction_def)
+apply(clarsimp simp add: instruction_simps)
+apply((sep_simp simp: evm_sep)+)
+apply(simp add: stateelm_means_simps stateelm_equiv_simps)
+			apply(simp add: rev_lookup)
+			apply(subst conj_commute)
+			apply(rule context_conjI)
+			 apply(rule conjI)
+			  apply(arith)
+			 apply(rule conjI)
+			  apply(simp add: short_rev_append rev_nth)
+			  apply(arith)
+				find_theorems name:comm "_\<and>_"
+			apply(erule_tac P="(_ \<and>* _)" in back_subst)
+apply(set_solve)
+				done
+  	
 lemma triple_inst_soundness:
 notes
   if_split[split del]
@@ -381,26 +825,51 @@ shows
   "triple_inst p i q \<Longrightarrow> triple_inst_sem p i q"
   apply(induction rule:triple_inst.induct)
       apply(erule triple_inst_arith.cases; clarsimp)
-          apply(simp add: inst_arith_2_1_low_sound)
-         apply(simp add: inst_arith_2_1_verylow_sound)
-        apply(simp add: inst_arith_3_1_sound)
-			 apply(inst_sound_set_eq simp: iszero_stack_def)
-       apply(set_solve)
-      apply(erule triple_inst_bits.cases; clarsimp)
-       apply(inst_sound_set_eq, set_solve)
-      apply(simp add: inst_bits_2_1_sound)
-     apply(erule triple_inst_misc.cases; clarsimp)
-     apply(simp only: inst_stop_sem)
+                       apply(inst_sound_set_eq, set_solve)
+                      apply(split if_split, rule conjI, rule impI)
+                      apply(inst_sound_set_eq, set_solve)+
+                     apply(split if_split, rule conjI, rule impI)
+                      apply(inst_sound_set_eq, set_solve)
+                     apply(inst_sound_set_eq, set_solve)
+                    apply(inst_sound_set_eq, set_solve)
+                   apply(inst_sound_set_eq, set_solve)
+                  apply(inst_sound_set_eq, set_solve)
+                 apply(inst_sound_set_eq, set_solve)
+                apply(inst_sound_set_eq, set_solve)
+               apply(split if_split, rule conjI, rule impI)
+                apply(inst_sound_set_eq, set_solve)
+               apply(inst_sound_set_eq, set_solve)
+              apply(split if_split, rule conjI, rule impI)
+               apply(inst_sound_set_eq, set_solve)
+              apply(inst_sound_set_eq, set_solve)
+             apply(inst_sound_set_eq simp: iszero_stack_def, set_solve)
+            apply(erule triple_inst_bits.cases; clarsimp)
+                apply(inst_sound_set_eq, set_solve)
+               apply(inst_sound_set_eq, set_solve)
+              apply(inst_sound_set_eq, set_solve)
+             apply(inst_sound_set_eq, set_solve)
+            apply(inst_sound_set_eq, set_solve)
+           apply(erule triple_inst_info.cases; clarsimp)
+  				 apply(inst_sound_set_eq, set_solve)
+   					 apply(erule triple_inst_memory.cases; clarsimp)
+  					  apply(rule inst_mload_sound[simplified])
+  					 apply(rule inst_mstore_sound[simplified])
+  					apply(erule triple_inst_misc.cases; clarsimp)
+  					 apply(rule inst_stop_sem)
+  					apply(rule inst_return_sem)
     apply(erule triple_inst_pc.cases; clarsimp)
      apply(inst_sound_set_eq, set_solve)
     apply(inst_sound_set_eq, set_solve)
    apply(erule triple_inst_stack.cases; clarsimp)
     apply(inst_sound_set_eq simp: constant_mark_def, set_solve)
-   apply(inst_sound_set_eq, set_solve)
-  apply(simp add: inst_swap_sound)
+    		apply(inst_sound_set_eq, set_solve)
+    apply(inst_sound_set_eq simp: cut_data_def, set_solve)
+    	apply(rule inst_swap_sound)
+  	 apply(rule inst_dup_sound)
+  	apply(inst_sound_set_eq, set_solve)
  apply(simp add: inst_strengthen_pre_sem)
 apply(simp add: inst_false_pre_sem)
-sorry
+done
 
 (* Soundness proof for triple_seq rules *)
 
@@ -1608,14 +2077,16 @@ lemma pc_before_inst:
 x = (n, i) \<Longrightarrow>
 pre s \<and> uniq_stateelm s \<Longrightarrow>
 PcElm n \<in> s"
-sorry
  apply(induct rule: triple_inst.induct; clarsimp)
-       apply(erule triple_inst_arith.cases; clarsimp; sep_simp simp: pure_sep sep_fun_simps; simp)
-      apply(erule triple_inst_bits.cases; clarsimp; sep_simp simp: pure_sep sep_fun_simps; simp)
-     apply(erule triple_inst_misc.cases; clarsimp; sep_simp simp: pure_sep sep_fun_simps; simp)
-    apply(erule triple_inst_pc.cases; clarsimp; sep_simp simp: pure_sep sep_fun_simps; simp)
-   apply(erule triple_inst_stack.cases; clarsimp; sep_simp simp: pure_sep sep_fun_simps; simp)
-  apply(sep_simp simp: pure_sep sep_fun_simps; simp)
+            apply(erule triple_inst_arith.cases; clarsimp; sep_simp simp: pure_sep sep_fun_simps; simp)
+           apply(erule triple_inst_bits.cases; clarsimp; sep_simp simp: pure_sep sep_fun_simps; simp)
+          apply(erule triple_inst_info.cases; clarsimp; sep_simp simp: pure_sep sep_fun_simps; simp)
+         apply(erule triple_inst_log.cases; clarsimp; sep_simp simp: pure_sep sep_fun_simps; simp)
+        apply(erule triple_inst_memory.cases; clarsimp; sep_simp simp: pure_sep sep_fun_simps; simp)
+       apply(erule triple_inst_misc.cases; clarsimp; sep_simp simp: pure_sep sep_fun_simps; simp)
+      apply(erule triple_inst_pc.cases; clarsimp; sep_simp simp: pure_sep sep_fun_simps; simp)
+     apply(erule triple_inst_stack.cases; clarsimp; sep_simp simp: pure_sep sep_fun_simps; simp)
+    apply(sep_simp simp: pure_sep sep_fun_simps; simp)+
  apply(simp add: pure_def)
 done
 
